# Linear Equations with Variables on Both Sides

When there are variables on both sides of an equivalency, we can manipulate both sides of the equation in a balanced way that makes it easier to solve.

We can look at the equation below to represent how adding or removing elements on each side of the equation in a balanced way will yield the correct result:

>2x + 3 = 5x - 2

This could otherwise be written as:

>x + x + 1 + 1 + 1 = x + x + x + x + x - 1 - 1

Since there are at least two x's on both sides of this equation, we can remove two x's from both sides with the following results:

>1 + 1 + 1 = x + x + x - 1 - 1

Otherwise written as:

>3 = 3x - 2

The next logical step would be to isolate the x variable. We can do this by subtracting adding two to both sides to negate the (-2) on the side of the equation with the x variable:

>3 = 3x - 2
>3 + 2 = 3x - 2 + 2
>5 = 3x

In order to progress in our task of isolating the x variable, we can then divide both sides by three:

>5 = 3x
>5 / 3 = 3x / 3

or

>5 / 3 = (3 / 3)x 

This will yield our solution for x:

>5 / 3 = x

### Least Common Multiple

The Least Common Multiple ( #LCM) is the smallest positive integer that is divisible by two or more numbers. When we are dealing with fractional values that are conflicting, we can multiply them by the LCM to find easier fractional values to work with, as seen below:

>3/4x + 2 = 3/8x -4

These fractions are not easily added together. We can transform them by multiplying both sides of the equation by the LCM of 8.

>8( 3/4x + 2) = 8(3/8x -4)

This simplifies to:

>6x + 16 = 3x - 32

### Variables as Denominator

In the cases where a variables is serving as the denominator of a fraction, we will need to use the LCM method applied to a variable instead of a constant.

>7 - (10 / x) = 2 + (15 / x)

We can then use the LCM method to create a linear form without fractions:

>x ( 7 - ( 10 / x )) = x (2 + (15 / x))

Which would yield:

>7x - ( x / 1 ) \* (10 / x ) = 2x + ( x / 1 ) \* (15 / x )

This simplifies to:

>7x - ( 10x / 1x ) = 2x + ( 15x / 1x )

Simplifying further to:

>7x -10 = 2x + 15

